systems/chord-util/LabeledMeasures.v
@@ -6,6 +6,7 @@ Require Import StructTact.FilterMap.
 Require Import InfSeqExt.infseq.
 Require Import Chord.InfSeqTactics.
 Require Import Chord.Chord.
+Require Import Chord.LabeledLemmas.
 
 (** This shouldn't live here but I'm not sure where it should live *)
 Lemma nat_strong_ind :
@@ -593,34 +594,6 @@ Section LocalMeasure.
       destruct hd eqn:?H.
       + firstorder.
       + exists hd; firstorder.
-  Qed.
-
-  Definition active_nodes (gst : global_state) :=
-    RemoveAll.remove_all addr_eq_dec (failed_nodes gst) (nodes gst).
-
-  Lemma labeled_step_dynamic_preserves_active_nodes :
-    forall gst l gst',
-      labeled_step_dynamic gst l gst' ->
-      active_nodes gst = active_nodes gst'.
-  Proof.
-    intros; unfold active_nodes.
-    erewrite labeled_step_dynamic_preserves_failed_nodes; eauto.
-    erewrite labeled_step_dynamic_preserves_nodes; eauto.
-  Qed.
-
-  Lemma active_nodes_always_identical :
-    forall l ex,
-      lb_execution ex ->
-      active_nodes (occ_gst (hd ex)) = l ->
-      always (fun ex' => l = active_nodes (occ_gst (hd ex'))) ex.
-  Proof.
-    cofix c. intros.
-    constructor; destruct ex.
-    - easy.
-    - apply c; eauto using lb_execution_invar.
-      inv_prop lb_execution.
-      find_apply_lem_hyp labeled_step_dynamic_preserves_active_nodes.
-      cbn; congruence.
   Qed.
 
   Definition global_measure (gst : global_state) : nat :=
