systems/chord-props/NodesHaveState.v
@@ -1,0 +1,113 @@
+Require Import List.
+
+Require Import StructTact.StructTactics.
+Require Import StructTact.Util.
+
+Require Import Chord.Chord.
+Require Import Chord.SystemReachable.
+
+Require Import Chord.SystemLemmas.
+Require Import Chord.HandlerLemmas.
+Require Import Chord.LabeledLemmas.
+
+Set Bullet Behavior "Strict Subproofs".
+
+Lemma run_init_for_creates_st :
+  forall l h gst,
+    NoDup l ->
+    In h l ->
+    In h (nodes (fold_left run_init_for l gst)) ->
+    exists st,
+      sigma (fold_left run_init_for l gst) h = Some st.
+Proof.
+  induction l; intros.
+  - easy.
+  - simpl in *.
+    break_or_hyp.
+    + unfold run_init_for.
+      assert (~ In h l)
+        by now apply NoDup_cons_iff.
+      rewrite fold_left_for_each_not_in;
+        eauto using sigma_apply_handler_result_diff.
+      destruct (start_handler h initial_nodes) as [[? ?] ?].
+      eauto using apply_handler_result_updates_sigma.
+    + eapply IHl; eauto.
+      eapply NoDup_cons_iff; eauto.
+Qed.
+
+Lemma in_run_init_for_nodes_in_l_or_acc :
+  forall l h gst,
+    In h (nodes (fold_left run_init_for l gst)) ->
+    In h l \/ In h (nodes gst).
+Proof.
+  induction l; intros.
+  - tauto.
+  - simpl in *.
+    find_apply_lem_hyp IHl.
+    unfold run_init_for in *.
+    erewrite <- apply_handler_result_preserves_nodes in * by eauto.
+    tauto.
+Qed.
+
+Lemma initial_st_node_in_initial_nodes :
+  forall h,
+    In h (nodes initial_st) ->
+    In h initial_nodes.
+Proof.
+  unfold initial_st.
+  intros.
+  find_apply_lem_hyp in_run_init_for_nodes_in_l_or_acc.
+  tauto.
+Qed.
+
+Theorem nodes_have_state_preserved :
+  forall gst gst',
+    (forall h, In h (nodes gst) -> exists st, sigma gst h = Some st) ->
+    step_dynamic gst gst' ->
+    (forall h, In h (nodes gst') -> exists st, sigma gst' h = Some st).
+Proof using.
+  intros.
+  break_step.
+  - destruct (addr_eq_dec h h0).
+    + subst_max.
+      apply update_for_start_sigma_h_exists.
+    + find_rewrite_lem update_for_start_nodes_eq.
+      find_apply_lem_hyp in_inv.
+      break_or_hyp; try (exfalso; eauto; fail).
+      find_apply_hyp_hyp.
+      break_exists_exists.
+      eapply update_for_start_sigma_h_n; eauto.
+  - eauto.
+  - destruct (addr_eq_dec h h0).
+    * eexists.
+      now apply update_eq.
+    * apply_prop_hyp In (In h).
+      break_exists_exists.
+      now eauto using sigma_ahr_passthrough.
+  - destruct (addr_eq_dec (fst (snd m)) h).
+    * eexists.
+      now apply update_eq.
+    * simpl.
+      find_apply_hyp_hyp.
+      break_exists_exists.
+      repeat find_reverse_rewrite.
+      now apply update_diff.
+  - admit.
+  - admit.
+Admitted.
+
+Lemma nodes_have_state :
+  forall gst h,
+    In h (nodes gst) ->
+    reachable_st gst ->
+    exists st,
+      sigma gst h = Some st.
+Proof.
+  intros.
+  generalize dependent h.
+  induct_reachable_st; intros.
+  - unfold initial_st in *.
+    apply run_init_for_creates_st;
+      eauto using initial_nodes_NoDup, initial_st_node_in_initial_nodes.
+  - eapply nodes_have_state_preserved; eauto.
+Qed.
